prepare some lemmas for instance list sema

polygen/InstanceListSema.v
@@ -88,6 +88,12 @@ Definition instr_point_sched_ltb (ip1 ip2: InstrPoint): bool :=
 Definition instr_point_sched_eqb (ip1 ip2: InstrPoint): bool := 
   comparison_eqb (lex_compare ip1.(ip_time_stamp) ip2.(ip_time_stamp)) Eq.
 
+Definition instr_point_sched_lt (ip1 ip2: InstrPoint): Prop := 
+  instr_point_sched_ltb ip1 ip2 = true. 
+
+Definition instr_point_sched_eq (ip1 ip2: InstrPoint): Prop := 
+  instr_point_sched_eqb ip1 ip2 = true. 
+
 
 Definition Permutable (ip1 ip2: InstrPoint) := 
     forall st1, 
@@ -174,5 +180,192 @@ Proof.
   eapply veq_refl.
 Qed.
 
+
+Require Import Setoid Morphisms.
+(* Require Import List. *)
+Require Import SetoidList.
+Require Import sflib.
+Require Import LibTactics.
+
+(* Require Import MSets. *)
+
+Require Import Sorting.Sorted.
+
+Instance ip_ts_eq: Equivalence instr_point_sched_eq.
+Proof.
+  constructor.
+  - intros x. unfold instr_point_sched_eq. 
+    unfold instr_point_sched_eqb.
+    rewrite lex_compare_reflexive. unfold comparison_eqb. simpl. trivial. 
+  - intros x y Hxy. unfold instr_point_sched_eq in *.
+    unfold instr_point_sched_eqb in *.  
+    rewrite lex_compare_antisym.  
+    rewrite comparison_eqb_iff_eq in Hxy.
+    rewrite Hxy. simpl. trivial.
+  - intros x y z Hxy Hyz. unfold instr_point_sched_eq in *. unfolds instr_point_sched_eqb.
+    rewrite  comparison_eqb_iff_eq in Hxy.
+    rewrite  comparison_eqb_iff_eq in Hyz.
+    rewrite  comparison_eqb_iff_eq.
+    eapply lex_compare_trans; eauto.
+Qed.
+
+
+Lemma instr_point_sched_le_antisym:
+forall x1 x2,
+instr_point_sched_le x1 x2 ->
+instr_point_sched_le x2 x1 ->
+instr_point_sched_eq x1 x2.
+Proof.
+  intros.
+  unfolds instr_point_sched_le.
+  unfold instr_point_sched_eq.
+  unfold instr_point_sched_eqb.
+  rewrite comparison_eqb_iff_eq.
+  destruct H; destruct H0; try contradiction; eauto.
+  - 
+  rewrite lex_compare_antisym in H.
+  rewrite H0 in H. 
+  unfold CompOpp in H. trivial.
+  discriminate.
+  - 
+  rewrite lex_compare_antisym in H.
+  rewrite H0 in H. 
+  unfold CompOpp in H. trivial.
+  discriminate.
+Qed.
+
+Lemma strongly_sorted_lists_by_timestamp_equal :
+  forall l1 l2,
+    StronglySorted instr_point_sched_le l1 ->
+    StronglySorted instr_point_sched_le l2 ->
+    NoDupA instr_point_sched_eq l1 ->
+    NoDupA instr_point_sched_eq l2 ->
+    (forall x, In x l1 <-> In x l2) ->
+    l1 = l2.
+Proof.
+  induction l1 as [|x1 l1 IH]; intros l2 Hs1 Hs2 Hnd1 Hnd2 Hin.
+  - destruct l2; [reflexivity |].
+    exfalso. apply (Hin i). apply in_eq.
+  - destruct l2 as [|x2 l2']; [> exfalso; apply (Hin x1); left; reflexivity |].
+    rename l1 into l1'.
+    assert (x1 = x2).
+    {
+      assert (Hin1: In x1 (x1:: l1')) by apply in_eq.
+      assert (Hin2: In x2 (x2 :: l2')) by apply in_eq.
+      assert (In x1 (x2 :: l2')). {
+        eapply Hin; eauto.
+      } 
+      destruct H as [Heq | Hin_tail]; symmetry; trivial.
+      - 
+
+        (* use NoDup to derive contradiction *)
+        assert (Hback: In x2 (x1 :: l1')). {
+          eapply Hin; eauto.
+        }
+        destruct Hback as [Heq' | Hin_tail'].
+        + symmetry in Heq'. trivial.
+        + 
+          assert (instr_point_sched_le x1 x2).
+          { 
+            inv Hs1.
+            eapply Forall_forall with (x:=x2) in H2; eauto.
+          }
+          assert (instr_point_sched_le x2 x1).
+          { 
+            inv Hs2.
+            eapply Forall_forall with (x:=x1) in H3; eauto.
+          }
+          assert (instr_point_sched_eq x1 x2). {
+            eapply instr_point_sched_le_antisym; eauto.
+          }
+          inv Hnd1.
+          eapply In_InA with (eqA:=instr_point_sched_eq) in Hin_tail'. 2: {eapply ip_ts_eq. }
+          clear - Hin_tail' H4 H1.
+          eapply InA_eqA with (y:=x1) in Hin_tail'; eauto.
+          {try contradiction. }
+          {eapply ip_ts_eq. }
+          {eapply ip_ts_eq. trivial. }
+    }
+    subst x2.
+    f_equal.
+    apply IH.
+    + eapply StronglySorted_inv; eauto.
+    + eapply StronglySorted_inv; eauto.
+    + 
+      replace l1' with ([] ++ l1'); trivial.
+      eapply NoDupA_split; eauto.
+    + 
+      replace l2' with ([] ++ l2'); trivial.
+      eapply NoDupA_split; eauto.
+    + intros x. split; intro Hx.
+      * assert (In x (x1 :: l1')). { eapply in_cons; trivial. }
+        eapply Hin in H; eauto.
+        destruct H as [Hx1 | Hx1].
+        -- subst. 
+          clear - Hnd1 Hx.
+          inv Hnd1. eapply In_InA with (eqA := instr_point_sched_eq ) in Hx; eauto. contradiction.
+          eapply ip_ts_eq.
+        -- trivial.
+      * assert (In x (x1 :: l2')). { eapply in_cons; trivial. }
+        eapply Hin in H; eauto.
+        destruct H as [Hx1 | Hx1].
+        -- subst. 
+          clear - Hnd2 Hx.
+          inv Hnd2. eapply In_InA with (eqA := instr_point_sched_eq ) in Hx; eauto. contradiction.
+          eapply ip_ts_eq.
+        -- trivial.   
+Qed.
+
+
+Lemma Sorted_incl_eq :
+  forall l1 l2,
+    Sorted instr_point_sched_le l1 ->
+    Sorted instr_point_sched_le l2 ->
+    (forall x, In x l1 <-> In x l2) ->
+    NoDupA instr_point_sched_eq l1 ->
+    NoDupA instr_point_sched_eq l2 ->
+    l1 = l2.
+Proof.
+  intros l1 l2  Hs1 Hs2 Heq Hinj1 Hinj2.
+  pose proof instr_point_sched_le_trans as Htrans.
+  apply Sorted_StronglySorted in Hs1; auto.
+  apply Sorted_StronglySorted in Hs2; auto.
+  eapply strongly_sorted_lists_by_timestamp_equal; eauto.
+Qed.
+
+Lemma Sorted_same_ele_nodup_implies_sema_eq:
+  forall l1 l2 st1 st2,
+    Sorted instr_point_sched_le l1 ->
+    Sorted instr_point_sched_le l2 ->
+    NoDupA instr_point_sched_eq l1 ->
+    NoDupA instr_point_sched_eq l2 ->
+    (forall x, In x l1 <-> In x l2) ->
+    instr_point_list_semantics l1 st1 st2 -> 
+    instr_point_list_semantics l2 st1 st2.
+Proof.
+  intros l1 l2 st1 st2 Hs1 Hs2 Hd1 Hd2 Hin Hsem1.
+  assert (l1 = l2). 
+  { eapply Sorted_incl_eq; eauto. }
+  subst. trivial.
+Qed.
+
+Lemma Sorted_same_ele_nodup_implies_sema_eq_stable:
+  forall l1 l2 st1 st2 st1' st2',
+    Sorted instr_point_sched_le l1 ->
+    Sorted instr_point_sched_le l2 ->
+    NoDupA instr_point_sched_eq l1 ->
+    NoDupA instr_point_sched_eq l2 ->
+    (forall x, In x l1 <-> In x l2) ->
+    instr_point_list_semantics l1 st1 st2 -> 
+    State.eq st1 st1' ->
+    State.eq st2 st2' ->
+    instr_point_list_semantics l2 st1' st2'.
+Proof.
+  intros l1 l2 st1 st2 st1' st2' Hs1 Hs2 Hd1 Hd2 Hin Hsem1 Hst1 Hst2.
+  assert (l1 = l2). 
+  { eapply Sorted_incl_eq; eauto. } 
+  eapply instr_point_list_sema_stable_under_state_eq with (st1':=st1') (st2':=st2') in Hsem1; eauto. 
+  subst. trivial.
+Qed.
 
 End ILSema.
